@prefix : <http://www.semanticweb.org/andrej/ontologies/2024/9/untitled-ontology-17/> .
@prefix owl: <http://www.w3.org/2002/07/owl#> .
@prefix rdf: <http://www.w3.org/1999/02/22-rdf-syntax-ns#> .
@prefix xml: <http://www.w3.org/XML/1998/namespace> .
@prefix xsd: <http://www.w3.org/2001/XMLSchema#> .
@prefix rdfs: <http://www.w3.org/2000/01/rdf-schema#> .
@base <http://www.semanticweb.org/andrej/ontologies/2024/9/untitled-ontology-17/> .

<https://github.com/andrej-kocijan/opentelemetry-ontology> rdf:type owl:Ontology .

#################################################################
#    Object Properties
#################################################################

###  http://www.semanticweb.org/andrej/ontologies/2024/9/untitled-ontology-17/anyValueListElement
:anyValueListElement rdf:type owl:ObjectProperty ;
                     rdfs:subPropertyOf owl:topObjectProperty ;
                     rdfs:domain :AnyValueList ;
                     rdfs:range :AnyValue .


###  http://www.semanticweb.org/andrej/ontologies/2024/9/untitled-ontology-17/attribute
:attribute rdf:type owl:ObjectProperty ;
           rdfs:subPropertyOf owl:topObjectProperty ;
           rdfs:domain :InstrumentationScope ,
                       :LogRecord ,
                       :Resource ;
           rdfs:range :KeyValue .


###  http://www.semanticweb.org/andrej/ontologies/2024/9/untitled-ontology-17/body
:body rdf:type owl:ObjectProperty ;
      rdfs:domain :LogRecord ;
      rdfs:range :AnyValue .


###  http://www.semanticweb.org/andrej/ontologies/2024/9/untitled-ontology-17/keyValueListElement
:keyValueListElement rdf:type owl:ObjectProperty ;
                     rdfs:subPropertyOf owl:topObjectProperty ;
                     rdfs:domain :KeyValueList ;
                     rdfs:range :KeyValue .


###  http://www.semanticweb.org/andrej/ontologies/2024/9/untitled-ontology-17/keyValueValue
:keyValueValue rdf:type owl:ObjectProperty ;
               rdfs:subPropertyOf owl:topObjectProperty ;
               rdfs:domain :KeyValue ;
               rdfs:range :AnyValue .


###  http://www.semanticweb.org/andrej/ontologies/2024/9/untitled-ontology-17/logRecord
:logRecord rdf:type owl:ObjectProperty ;
           rdfs:domain :ScopeLogs ;
           rdfs:range :LogRecord .


###  http://www.semanticweb.org/andrej/ontologies/2024/9/untitled-ontology-17/resource
:resource rdf:type owl:ObjectProperty ;
          rdfs:domain :ResourceLogs ;
          rdfs:range :Resource .


###  http://www.semanticweb.org/andrej/ontologies/2024/9/untitled-ontology-17/resourceLogs
:resourceLogs rdf:type owl:ObjectProperty ;
              rdfs:domain :LogsData ;
              rdfs:range :ResourceLogs .


###  http://www.semanticweb.org/andrej/ontologies/2024/9/untitled-ontology-17/scope
:scope rdf:type owl:ObjectProperty ;
       rdfs:domain :ScopeLogs ;
       rdfs:range :InstrumentationScope .


###  http://www.semanticweb.org/andrej/ontologies/2024/9/untitled-ontology-17/scopeLogs
:scopeLogs rdf:type owl:ObjectProperty ;
           rdfs:domain :ResourceLogs ;
           rdfs:range :ScopeLogs .


###  http://www.semanticweb.org/andrej/ontologies/2024/9/untitled-ontology-17/severitryNumber
:severitryNumber rdf:type owl:ObjectProperty ;
                 rdfs:domain :LogRecord ;
                 rdfs:range :SeverityNumber .


#################################################################
#    Data properties
#################################################################

###  http://www.semanticweb.org/andrej/ontologies/2024/9/untitled-ontology-17/droppedAttributesCount
:droppedAttributesCount rdf:type owl:DatatypeProperty ;
                        rdfs:subPropertyOf owl:topDataProperty ;
                        rdfs:domain :InstrumentationScope ,
                                    :LogRecord ,
                                    :Resource ;
                        rdfs:range xsd:unsignedInt ;
                        rdfs:comment "droppedAttributesCount is the number of dropped attributes. If the value is 0, then no attributes were dropped."@en .


###  http://www.semanticweb.org/andrej/ontologies/2024/9/untitled-ontology-17/enumOptionValue
:enumOptionValue rdf:type owl:DatatypeProperty ;
                 rdfs:domain :Enum .


###  http://www.semanticweb.org/andrej/ontologies/2024/9/untitled-ontology-17/flags
:flags rdf:type owl:DatatypeProperty ;
       rdfs:subPropertyOf owl:topDataProperty ;
       rdfs:domain :LogRecord ;
       rdfs:range xsd:unsignedInt ;
       rdfs:comment "Flags, a bit field. 8 least significant bits are the trace flags as defined in W3C Trace Context specification. 24 most significant bits are reserved and must be set to 0. Readers must not assume that 24 most significant bits will be zero and must correctly mask the bits when reading 8-bit trace flag (use flags & LOG_RECORD_FLAGS_TRACE_FLAGS_MASK). [Optional]."@en .


###  http://www.semanticweb.org/andrej/ontologies/2024/9/untitled-ontology-17/keyValueKey
:keyValueKey rdf:type owl:DatatypeProperty ;
             rdfs:subPropertyOf owl:topDataProperty ;
             rdfs:domain :KeyValue ;
             rdfs:range xsd:string .


###  http://www.semanticweb.org/andrej/ontologies/2024/9/untitled-ontology-17/name
:name rdf:type owl:DatatypeProperty ;
      rdfs:subPropertyOf owl:topDataProperty ;
      rdfs:domain :InstrumentationScope ;
      rdfs:range xsd:string ;
      rdfs:comment "An empty instrumentation scope name means the name is unknown."@en .


###  http://www.semanticweb.org/andrej/ontologies/2024/9/untitled-ontology-17/observedTimeUnixNano
:observedTimeUnixNano rdf:type owl:DatatypeProperty ;
                      rdfs:subPropertyOf owl:topDataProperty ;
                      rdfs:domain :LogRecord ;
                      rdfs:range xsd:unsignedLong ;
                      rdfs:comment """Time when the event was observed by the collection system.
For events that originate in OpenTelemetry (e.g. using OpenTelemetry Logging SDK) this timestamp is typically set at the generation time and is equal to Timestamp.
For events originating externally and collected by OpenTelemetry (e.g. using Collector) this is the time when OpenTelemetry's code observed the event measured by the clock of the OpenTelemetry code. This field MUST be set once the event is observed by OpenTelemetry.

For converting OpenTelemetry log data to formats that support only one timestamp or when receiving OpenTelemetry log data by recipients that support only one timestamp internally the following logic is recommended:
  - Use time_unix_nano if it is present, otherwise use observed_time_unix_nano.

Value is UNIX Epoch time in nanoseconds since 00:00:00 UTC on 1 January 1970.
Value of 0 indicates unknown or missing timestamp.""" .


###  http://www.semanticweb.org/andrej/ontologies/2024/9/untitled-ontology-17/primitiveValueValue
:primitiveValueValue rdf:type owl:DatatypeProperty ;
                     rdfs:domain :PrimitiveValue ;
                     rdfs:range xsd:boolean ,
                                xsd:byte ,
                                xsd:double ,
                                xsd:int ,
                                xsd:string .


###  http://www.semanticweb.org/andrej/ontologies/2024/9/untitled-ontology-17/schemaUrl
:schemaUrl rdf:type owl:DatatypeProperty ;
           rdfs:domain :ResourceLogs ,
                       :ScopeLogs ;
           rdfs:range xsd:string ;
           rdfs:comment """The Schema URL, if known. This is the identifier of the Schema that the log data is recorded in. To learn more about Schema URL see https://opentelemetry.io/docs/specs/otel/schemas/#schema-url
This schema_url applies to all logs in the \"logs\" field."""@en .


###  http://www.semanticweb.org/andrej/ontologies/2024/9/untitled-ontology-17/severityText
:severityText rdf:type owl:DatatypeProperty ;
              rdfs:domain :LogRecord ;
              rdfs:range xsd:string ;
              rdfs:comment "The severity text (also known as log level). The original string representation as it is known at the source. [Optional]." .


###  http://www.semanticweb.org/andrej/ontologies/2024/9/untitled-ontology-17/spanId
:spanId rdf:type owl:DatatypeProperty ;
        rdfs:subPropertyOf owl:topDataProperty ;
        rdfs:domain :LogRecord ;
        rdfs:range xsd:byte ;
        rdfs:comment """A unique identifier for a span within a trace, assigned when the span
is created. The ID is an 8-byte array. An ID with all zeroes OR of length
other than 8 bytes is considered invalid (empty string in OTLP/JSON
is zero-length and thus is also invalid).

This field is optional. If the sender specifies a valid span_id then it SHOULD also
specify a valid trace_id.

The receivers SHOULD assume that the log record is not associated with a
span if any of the following is true:
  - the field is not present,
  - the field contains an invalid value.""" .


###  http://www.semanticweb.org/andrej/ontologies/2024/9/untitled-ontology-17/timeUnixNano
:timeUnixNano rdf:type owl:DatatypeProperty ;
              rdfs:subPropertyOf owl:topDataProperty ;
              rdfs:domain :LogRecord ;
              rdfs:range xsd:unsignedLong ;
              rdfs:comment """timeUnixNano is the time when the event occurred.
Value is UNIX Epoch time in nanoseconds since 00:00:00 UTC on 1 January 1970.
Value of 0 indicates unknown or missing timestamp."""@en .


###  http://www.semanticweb.org/andrej/ontologies/2024/9/untitled-ontology-17/traceId
:traceId rdf:type owl:DatatypeProperty ;
         rdfs:subPropertyOf owl:topDataProperty ;
         rdfs:domain :LogRecord ;
         rdfs:range xsd:byte ;
         rdfs:comment """A unique identifier for a trace. All logs from the same trace share
the same `trace_id`. The ID is a 16-byte array. An ID with all zeroes OR
of length other than 16 bytes is considered invalid (empty string in OTLP/JSON
is zero-length and thus is also invalid).

This field is optional.

The receivers SHOULD assume that the log record is not associated with a
trace if any of the following is true:
  - the field is not present,
  - the field contains an invalid value."""@en .


###  http://www.semanticweb.org/andrej/ontologies/2024/9/untitled-ontology-17/version
:version rdf:type owl:DatatypeProperty ;
         rdfs:subPropertyOf owl:topDataProperty ;
         rdfs:domain :InstrumentationScope ;
         rdfs:range xsd:string .


#################################################################
#    Classes
#################################################################

###  http://www.semanticweb.org/andrej/ontologies/2024/9/untitled-ontology-17/AnyValue
:AnyValue rdf:type owl:Class ;
          rdfs:comment "AnyValue is used to represent any type of attribute value. AnyValue may contain a primitive value such as a string or integer or it may contain an arbitrary nested object containing arrays, key-value lists and primitives."@en .


###  http://www.semanticweb.org/andrej/ontologies/2024/9/untitled-ontology-17/AnyValueList
:AnyValueList rdf:type owl:Class ;
              rdfs:subClassOf :AnyValue .


###  http://www.semanticweb.org/andrej/ontologies/2024/9/untitled-ontology-17/Enum
:Enum rdf:type owl:Class ;
      rdfs:subClassOf [ rdf:type owl:Restriction ;
                        owl:onProperty :enumOptionValue ;
                        owl:qualifiedCardinality "1"^^xsd:nonNegativeInteger ;
                        owl:onDataRange xsd:int
                      ] .


###  http://www.semanticweb.org/andrej/ontologies/2024/9/untitled-ontology-17/InstrumentationScope
:InstrumentationScope rdf:type owl:Class ;
                      rdfs:subClassOf [ rdf:type owl:Restriction ;
                                        owl:onProperty :droppedAttributesCount ;
                                        owl:qualifiedCardinality "1"^^xsd:nonNegativeInteger ;
                                        owl:onDataRange xsd:unsignedInt
                                      ] ,
                                      [ rdf:type owl:Restriction ;
                                        owl:onProperty :version ;
                                        owl:qualifiedCardinality "1"^^xsd:nonNegativeInteger ;
                                        owl:onDataRange xsd:string
                                      ] ,
                                      [ rdf:type owl:Restriction ;
                                        owl:onProperty :name ;
                                        owl:maxQualifiedCardinality "1"^^xsd:nonNegativeInteger ;
                                        owl:onDataRange xsd:string
                                      ] ;
                      rdfs:comment "InstrumentationScope is a message representing the instrumentation scope information such as the fully qualified name and version." .


###  http://www.semanticweb.org/andrej/ontologies/2024/9/untitled-ontology-17/KeyValue
:KeyValue rdf:type owl:Class ;
          rdfs:subClassOf :AnyValue ,
                          [ rdf:type owl:Restriction ;
                            owl:onProperty :keyValueValue ;
                            owl:qualifiedCardinality "1"^^xsd:nonNegativeInteger ;
                            owl:onClass :AnyValue
                          ] ,
                          [ rdf:type owl:Restriction ;
                            owl:onProperty :keyValueKey ;
                            owl:qualifiedCardinality "1"^^xsd:nonNegativeInteger ;
                            owl:onDataRange xsd:string
                          ] ;
          rdfs:comment "KeyValue is a key-value pair that is used to store Span attributes, Link attributes, etc."@en .


###  http://www.semanticweb.org/andrej/ontologies/2024/9/untitled-ontology-17/KeyValueList
:KeyValueList rdf:type owl:Class ;
              rdfs:subClassOf :AnyValue .


###  http://www.semanticweb.org/andrej/ontologies/2024/9/untitled-ontology-17/LogRecord
:LogRecord rdf:type owl:Class ;
           rdfs:subClassOf [ rdf:type owl:Restriction ;
                             owl:onProperty :severitryNumber ;
                             owl:maxQualifiedCardinality "1"^^xsd:nonNegativeInteger ;
                             owl:onClass :SeverityNumber
                           ] ,
                           [ rdf:type owl:Restriction ;
                             owl:onProperty :droppedAttributesCount ;
                             owl:qualifiedCardinality "1"^^xsd:nonNegativeInteger ;
                             owl:onDataRange xsd:unsignedInt
                           ] ,
                           [ rdf:type owl:Restriction ;
                             owl:onProperty :flags ;
                             owl:maxQualifiedCardinality "1"^^xsd:nonNegativeInteger ;
                             owl:onDataRange xsd:unsignedInt
                           ] ,
                           [ rdf:type owl:Restriction ;
                             owl:onProperty :observedTimeUnixNano ;
                             owl:maxQualifiedCardinality "1"^^xsd:nonNegativeInteger ;
                             owl:onDataRange xsd:unsignedLong
                           ] ,
                           [ rdf:type owl:Restriction ;
                             owl:onProperty :severityText ;
                             owl:maxQualifiedCardinality "1"^^xsd:nonNegativeInteger ;
                             owl:onDataRange xsd:string
                           ] ,
                           [ rdf:type owl:Restriction ;
                             owl:onProperty :spanId ;
                             owl:maxQualifiedCardinality "1"^^xsd:nonNegativeInteger ;
                             owl:onDataRange xsd:byte
                           ] ,
                           [ rdf:type owl:Restriction ;
                             owl:onProperty :timeUnixNano ;
                             owl:maxQualifiedCardinality "1"^^xsd:nonNegativeInteger ;
                             owl:onDataRange xsd:unsignedLong
                           ] ,
                           [ rdf:type owl:Restriction ;
                             owl:onProperty :traceId ;
                             owl:maxQualifiedCardinality "1"^^xsd:nonNegativeInteger ;
                             owl:onDataRange xsd:byte
                           ] ;
           rdfs:comment """A log record according to OpenTelemetry Log Data Model:
https://github.com/open-telemetry/oteps/blob/main/text/logs/0097-log-data-model.md"""@en .


###  http://www.semanticweb.org/andrej/ontologies/2024/9/untitled-ontology-17/LogRecordFlags
:LogRecordFlags rdf:type owl:Class ;
                owl:equivalentClass [ rdf:type owl:Class ;
                                      owl:oneOf ( :LOG_RECORD_FLAGS_DO_NOT_USE
                                                  :LOG_RECORD_FLAGS_TRACE_FLAGS_MASK
                                                )
                                    ] ;
                rdfs:subClassOf :Enum ;
                rdfs:comment """The zero value for the enum. Should not be used for comparisons.
Instead use bitwise \"and\" with the appropriate mask as shown above.

Bits 0-7 are used for trace flags.

Bits 8-31 are reserved for future use."""@en .


###  http://www.semanticweb.org/andrej/ontologies/2024/9/untitled-ontology-17/LogsData
:LogsData rdf:type owl:Class ;
          rdfs:subClassOf [ rdf:type owl:Restriction ;
                            owl:onProperty :resourceLogs ;
                            owl:minQualifiedCardinality "0"^^xsd:nonNegativeInteger ;
                            owl:onClass :ResourceLogs
                          ] ;
          rdfs:comment """LogsData represents the logs data that can be stored in a persistent storage, OR can be embedded by other protocols that transfer OTLP logs data but do not implement the OTLP protocol.

The main difference between this message and collector protocol is that in this message there will not be any \"control\" or \"metadata\" specific to OTLP protocol.

When new fields are added into this message, the OTLP request MUST be updated as well."""@en .


###  http://www.semanticweb.org/andrej/ontologies/2024/9/untitled-ontology-17/PrimitiveValue
:PrimitiveValue rdf:type owl:Class ;
                rdfs:subClassOf :AnyValue ,
                                [ rdf:type owl:Restriction ;
                                  owl:onProperty :primitiveValueValue ;
                                  owl:qualifiedCardinality "1"^^xsd:nonNegativeInteger ;
                                  owl:onDataRange [ rdf:type rdfs:Datatype ;
                                                    owl:unionOf ( xsd:boolean
                                                                  xsd:byte
                                                                  xsd:double
                                                                  xsd:int
                                                                  xsd:string
                                                                )
                                                  ]
                                ] .


###  http://www.semanticweb.org/andrej/ontologies/2024/9/untitled-ontology-17/Resource
:Resource rdf:type owl:Class ;
          rdfs:subClassOf [ rdf:type owl:Restriction ;
                            owl:onProperty :droppedAttributesCount ;
                            owl:qualifiedCardinality "1"^^xsd:nonNegativeInteger ;
                            owl:onDataRange xsd:unsignedInt
                          ] ;
          rdfs:comment "Resource information."@en .


###  http://www.semanticweb.org/andrej/ontologies/2024/9/untitled-ontology-17/ResourceLogs
:ResourceLogs rdf:type owl:Class ;
              rdfs:subClassOf [ rdf:type owl:Restriction ;
                                owl:onProperty :scopeLogs ;
                                owl:minQualifiedCardinality "0"^^xsd:nonNegativeInteger ;
                                owl:onClass :ScopeLogs
                              ] ,
                              [ rdf:type owl:Restriction ;
                                owl:onProperty :resource ;
                                owl:maxQualifiedCardinality "1"^^xsd:nonNegativeInteger ;
                                owl:onClass :Resource
                              ] ,
                              [ rdf:type owl:Restriction ;
                                owl:onProperty :schemaUrl ;
                                owl:maxQualifiedCardinality "1"^^xsd:nonNegativeInteger ;
                                owl:onDataRange xsd:string
                              ] ;
              rdfs:comment "A collection of ScopeLogs from a Resource." .


###  http://www.semanticweb.org/andrej/ontologies/2024/9/untitled-ontology-17/ScopeLogs
:ScopeLogs rdf:type owl:Class ;
           rdfs:subClassOf [ rdf:type owl:Restriction ;
                             owl:onProperty :logRecord ;
                             owl:minQualifiedCardinality "0"^^xsd:nonNegativeInteger ;
                             owl:onClass :LogRecord
                           ] ,
                           [ rdf:type owl:Restriction ;
                             owl:onProperty :scope ;
                             owl:maxQualifiedCardinality "1"^^xsd:nonNegativeInteger ;
                             owl:onClass :InstrumentationScope
                           ] ,
                           [ rdf:type owl:Restriction ;
                             owl:onProperty :schemaUrl ;
                             owl:maxQualifiedCardinality "1"^^xsd:nonNegativeInteger ;
                             owl:onDataRange xsd:string
                           ] ;
           rdfs:comment "A collection of Logs produced by a Scope." .


###  http://www.semanticweb.org/andrej/ontologies/2024/9/untitled-ontology-17/SeverityNumber
:SeverityNumber rdf:type owl:Class ;
                owl:equivalentClass [ rdf:type owl:Class ;
                                      owl:oneOf ( :SEVERITY_NUMBER_DEBUG
                                                  :SEVERITY_NUMBER_DEBUG2
                                                  :SEVERITY_NUMBER_DEBUG3
                                                  :SEVERITY_NUMBER_DEBUG4
                                                  :SEVERITY_NUMBER_ERROR
                                                  :SEVERITY_NUMBER_ERROR2
                                                  :SEVERITY_NUMBER_ERROR3
                                                  :SEVERITY_NUMBER_ERROR4
                                                  :SEVERITY_NUMBER_FATAL
                                                  :SEVERITY_NUMBER_FATAL2
                                                  :SEVERITY_NUMBER_FATAL3
                                                  :SEVERITY_NUMBER_FATAL4
                                                  :SEVERITY_NUMBER_INFO
                                                  :SEVERITY_NUMBER_INFO2
                                                  :SEVERITY_NUMBER_INFO3
                                                  :SEVERITY_NUMBER_INFO4
                                                  :SEVERITY_NUMBER_TRACE
                                                  :SEVERITY_NUMBER_TRACE2
                                                  :SEVERITY_NUMBER_TRACE3
                                                  :SEVERITY_NUMBER_TRACE4
                                                  :SEVERITY_NUMBER_UNSPECIFIED
                                                  :SEVERITY_NUMBER_WARN
                                                  :SEVERITY_NUMBER_WARN2
                                                  :SEVERITY_NUMBER_WARN3
                                                  :SEVERITY_NUMBER_WARN4
                                                )
                                    ] ;
                rdfs:subClassOf :Enum ;
                rdfs:comment "Possible values for LogRecord.SeverityNumber."@en .


###  https://github.com/andrej-kocijan/opentelemetry-ontology#SpanFlags
:SpanFlags rdf:type owl:Class ;
           owl:equivalentClass [ rdf:type owl:Class ;
                                 owl:oneOf ( :SPAN_FLAGS_CONTEXT_HAS_IS_REMOTE_MASK
                                             :SPAN_FLAGS_CONTEXT_IS_REMOTE_MASK
                                             :SPAN_FLAGS_DO_NOT_USE
                                             :SPAN_FLAGS_TRACE_FLAGS_MASK
                                           )
                               ] ;
           rdfs:subClassOf :Enum ;
           rdfs:comment """The zero value for the enum. Should not be used for comparisons.
Instead use bitwise \"and\" with the appropriate mask as shown above.

Bits 0-7 are used for trace flags.

Bits 8 and 9 are used to indicate that the parent span or link span is remote.
Bit 8 (`HAS_IS_REMOTE`) indicates whether the value is known.
Bit 9 (`IS_REMOTE`) indicates whether the span or link is remote.

Bits 10-31 are reserved for future use.""" .


###  https://github.com/andrej-kocijan/opentelemetry-ontology#SpanKind
:SpanKind rdf:type owl:Class ;
          owl:equivalentClass [ rdf:type owl:Class ;
                                owl:oneOf ( :SPAN_KIND_CLIENT
                                            :SPAN_KIND_CONSUMER
                                            :SPAN_KIND_INTERNAL
                                            :SPAN_KIND_PRODUCER
                                            :SPAN_KIND_SERVER
                                            :SPAN_KIND_UNSPECIFIED
                                          )
                              ] ;
          rdfs:subClassOf :Enum ;
          rdfs:comment "SpanKind is the type of span. Can be used to specify additional relationships between spans in addition to a parent/child relationship."@en .


###  https://github.com/andrej-kocijan/opentelemetry-ontology#StatusCode
:StatusCode rdf:type owl:Class ;
            owl:equivalentClass [ rdf:type owl:Class ;
                                  owl:oneOf ( :STATUS_CODE_ERROR
                                              :STATUS_CODE_OK
                                              :STATUS_CODE_UNSET
                                            )
                                ] ;
            rdfs:subClassOf :Enum ;
            rdfs:comment "For the semantics of status codes see https://github.com/open-telemetry/opentelemetry-specification/blob/main/specification/trace/api.md#set-status"@en .


#################################################################
#    Individuals
#################################################################

###  http://www.semanticweb.org/andrej/ontologies/2024/9/untitled-ontology-17/LOG_RECORD_FLAGS_DO_NOT_USE
:LOG_RECORD_FLAGS_DO_NOT_USE rdf:type owl:NamedIndividual ,
                                      :LogRecordFlags ;
                             :enumOptionValue "0"^^xsd:int .


###  http://www.semanticweb.org/andrej/ontologies/2024/9/untitled-ontology-17/LOG_RECORD_FLAGS_TRACE_FLAGS_MASK
:LOG_RECORD_FLAGS_TRACE_FLAGS_MASK rdf:type owl:NamedIndividual ,
                                            :LogRecordFlags .


###  http://www.semanticweb.org/andrej/ontologies/2024/9/untitled-ontology-17/SEVERITY_NUMBER_DEBUG
:SEVERITY_NUMBER_DEBUG rdf:type owl:NamedIndividual ,
                                :SeverityNumber ;
                       :enumOptionValue "5"^^xsd:int .


###  http://www.semanticweb.org/andrej/ontologies/2024/9/untitled-ontology-17/SEVERITY_NUMBER_DEBUG2
:SEVERITY_NUMBER_DEBUG2 rdf:type owl:NamedIndividual ,
                                 :SeverityNumber ;
                        :enumOptionValue "6"^^xsd:int .


###  http://www.semanticweb.org/andrej/ontologies/2024/9/untitled-ontology-17/SEVERITY_NUMBER_DEBUG3
:SEVERITY_NUMBER_DEBUG3 rdf:type owl:NamedIndividual ,
                                 :SeverityNumber ;
                        :enumOptionValue "7"^^xsd:int .


###  http://www.semanticweb.org/andrej/ontologies/2024/9/untitled-ontology-17/SEVERITY_NUMBER_DEBUG4
:SEVERITY_NUMBER_DEBUG4 rdf:type owl:NamedIndividual ,
                                 :SeverityNumber ;
                        :enumOptionValue "8"^^xsd:int .


###  http://www.semanticweb.org/andrej/ontologies/2024/9/untitled-ontology-17/SEVERITY_NUMBER_ERROR
:SEVERITY_NUMBER_ERROR rdf:type owl:NamedIndividual ,
                                :SeverityNumber ;
                       :enumOptionValue "17"^^xsd:int .


###  http://www.semanticweb.org/andrej/ontologies/2024/9/untitled-ontology-17/SEVERITY_NUMBER_ERROR2
:SEVERITY_NUMBER_ERROR2 rdf:type owl:NamedIndividual ,
                                 :SeverityNumber ;
                        :enumOptionValue "18"^^xsd:int .


###  http://www.semanticweb.org/andrej/ontologies/2024/9/untitled-ontology-17/SEVERITY_NUMBER_ERROR3
:SEVERITY_NUMBER_ERROR3 rdf:type owl:NamedIndividual ,
                                 :SeverityNumber ;
                        :enumOptionValue "19"^^xsd:int .


###  http://www.semanticweb.org/andrej/ontologies/2024/9/untitled-ontology-17/SEVERITY_NUMBER_ERROR4
:SEVERITY_NUMBER_ERROR4 rdf:type owl:NamedIndividual ,
                                 :SeverityNumber ;
                        :enumOptionValue "20"^^xsd:int .


###  http://www.semanticweb.org/andrej/ontologies/2024/9/untitled-ontology-17/SEVERITY_NUMBER_FATAL
:SEVERITY_NUMBER_FATAL rdf:type owl:NamedIndividual ,
                                :SeverityNumber ;
                       :enumOptionValue "21"^^xsd:int .


###  http://www.semanticweb.org/andrej/ontologies/2024/9/untitled-ontology-17/SEVERITY_NUMBER_FATAL2
:SEVERITY_NUMBER_FATAL2 rdf:type owl:NamedIndividual ,
                                 :SeverityNumber ;
                        :enumOptionValue "22"^^xsd:int .


###  http://www.semanticweb.org/andrej/ontologies/2024/9/untitled-ontology-17/SEVERITY_NUMBER_FATAL3
:SEVERITY_NUMBER_FATAL3 rdf:type owl:NamedIndividual ,
                                 :SeverityNumber ;
                        :enumOptionValue "23"^^xsd:int .


###  http://www.semanticweb.org/andrej/ontologies/2024/9/untitled-ontology-17/SEVERITY_NUMBER_FATAL4
:SEVERITY_NUMBER_FATAL4 rdf:type owl:NamedIndividual ,
                                 :SeverityNumber ;
                        :enumOptionValue "24"^^xsd:int .


###  http://www.semanticweb.org/andrej/ontologies/2024/9/untitled-ontology-17/SEVERITY_NUMBER_INFO
:SEVERITY_NUMBER_INFO rdf:type owl:NamedIndividual ,
                               :SeverityNumber ;
                      :enumOptionValue "9"^^xsd:int .


###  http://www.semanticweb.org/andrej/ontologies/2024/9/untitled-ontology-17/SEVERITY_NUMBER_INFO2
:SEVERITY_NUMBER_INFO2 rdf:type owl:NamedIndividual ,
                                :SeverityNumber ;
                       :enumOptionValue "10"^^xsd:int .


###  http://www.semanticweb.org/andrej/ontologies/2024/9/untitled-ontology-17/SEVERITY_NUMBER_INFO3
:SEVERITY_NUMBER_INFO3 rdf:type owl:NamedIndividual ,
                                :SeverityNumber ;
                       :enumOptionValue "11"^^xsd:int .


###  http://www.semanticweb.org/andrej/ontologies/2024/9/untitled-ontology-17/SEVERITY_NUMBER_INFO4
:SEVERITY_NUMBER_INFO4 rdf:type owl:NamedIndividual ,
                                :SeverityNumber ;
                       :enumOptionValue "12"^^xsd:int .


###  http://www.semanticweb.org/andrej/ontologies/2024/9/untitled-ontology-17/SEVERITY_NUMBER_TRACE
:SEVERITY_NUMBER_TRACE rdf:type owl:NamedIndividual ,
                                :SeverityNumber ;
                       :enumOptionValue "1"^^xsd:int .


###  http://www.semanticweb.org/andrej/ontologies/2024/9/untitled-ontology-17/SEVERITY_NUMBER_TRACE2
:SEVERITY_NUMBER_TRACE2 rdf:type owl:NamedIndividual ,
                                 :SeverityNumber ;
                        :enumOptionValue "2"^^xsd:int .


###  http://www.semanticweb.org/andrej/ontologies/2024/9/untitled-ontology-17/SEVERITY_NUMBER_TRACE3
:SEVERITY_NUMBER_TRACE3 rdf:type owl:NamedIndividual ,
                                 :SeverityNumber ;
                        :enumOptionValue "3"^^xsd:int .


###  http://www.semanticweb.org/andrej/ontologies/2024/9/untitled-ontology-17/SEVERITY_NUMBER_TRACE4
:SEVERITY_NUMBER_TRACE4 rdf:type owl:NamedIndividual ,
                                 :SeverityNumber ;
                        :enumOptionValue "4"^^xsd:int .


###  http://www.semanticweb.org/andrej/ontologies/2024/9/untitled-ontology-17/SEVERITY_NUMBER_UNSPECIFIED
:SEVERITY_NUMBER_UNSPECIFIED rdf:type owl:NamedIndividual ,
                                      :SeverityNumber ;
                             :enumOptionValue "0"^^xsd:int .


###  http://www.semanticweb.org/andrej/ontologies/2024/9/untitled-ontology-17/SEVERITY_NUMBER_WARN
:SEVERITY_NUMBER_WARN rdf:type owl:NamedIndividual ,
                               :SeverityNumber ;
                      :enumOptionValue "13"^^xsd:int .


###  http://www.semanticweb.org/andrej/ontologies/2024/9/untitled-ontology-17/SEVERITY_NUMBER_WARN2
:SEVERITY_NUMBER_WARN2 rdf:type owl:NamedIndividual ,
                                :SeverityNumber ;
                       :enumOptionValue "14"^^xsd:int .


###  http://www.semanticweb.org/andrej/ontologies/2024/9/untitled-ontology-17/SEVERITY_NUMBER_WARN3
:SEVERITY_NUMBER_WARN3 rdf:type owl:NamedIndividual ,
                                :SeverityNumber ;
                       :enumOptionValue "15"^^xsd:int .


###  http://www.semanticweb.org/andrej/ontologies/2024/9/untitled-ontology-17/SEVERITY_NUMBER_WARN4
:SEVERITY_NUMBER_WARN4 rdf:type owl:NamedIndividual ,
                                :SeverityNumber ;
                       :enumOptionValue "16"^^xsd:int .


###  https://github.com/andrej-kocijan/opentelemetry-ontology#SPAN_FLAGS_CONTEXT_HAS_IS_REMOTE_MASK
:SPAN_FLAGS_CONTEXT_HAS_IS_REMOTE_MASK rdf:type owl:NamedIndividual ,
                                                :SpanFlags ;
                                       :enumOptionValue "256"^^xsd:int .


###  https://github.com/andrej-kocijan/opentelemetry-ontology#SPAN_FLAGS_CONTEXT_IS_REMOTE_MASK
:SPAN_FLAGS_CONTEXT_IS_REMOTE_MASK rdf:type owl:NamedIndividual ,
                                            :SpanFlags ;
                                   :enumOptionValue "512"^^xsd:int .


###  https://github.com/andrej-kocijan/opentelemetry-ontology#SPAN_FLAGS_DO_NOT_USE
:SPAN_FLAGS_DO_NOT_USE rdf:type owl:NamedIndividual ,
                                :SpanFlags ;
                       :enumOptionValue "0"^^xsd:int .


###  https://github.com/andrej-kocijan/opentelemetry-ontology#SPAN_FLAGS_TRACE_FLAGS_MASK
:SPAN_FLAGS_TRACE_FLAGS_MASK rdf:type owl:NamedIndividual ,
                                      :SpanFlags ;
                             :enumOptionValue "255"^^xsd:int .


###  https://github.com/andrej-kocijan/opentelemetry-ontology#SPAN_KIND_CLIENT
:SPAN_KIND_CLIENT rdf:type owl:NamedIndividual ,
                           :SpanKind ;
                  :enumOptionValue "3"^^xsd:int ;
                  rdfs:comment "Indicates that the span describes a request to some remote service."@en .


###  https://github.com/andrej-kocijan/opentelemetry-ontology#SPAN_KIND_CONSUMER
:SPAN_KIND_CONSUMER rdf:type owl:NamedIndividual ,
                             :SpanKind ;
                    :enumOptionValue "5"^^xsd:int ;
                    rdfs:comment """Indicates that the span describes consumer receiving a message from a broker.
Like the PRODUCER kind, there is often no direct critical path latency relationship between producer and consumer spans."""@en .


###  https://github.com/andrej-kocijan/opentelemetry-ontology#SPAN_KIND_INTERNAL
:SPAN_KIND_INTERNAL rdf:type owl:NamedIndividual ,
                             :SpanKind ;
                    :enumOptionValue "1"^^xsd:int ;
                    rdfs:comment "Indicates that the span represents an internal operation within an application, as opposed to an operation happening at the boundaries. Default value."@en .


###  https://github.com/andrej-kocijan/opentelemetry-ontology#SPAN_KIND_PRODUCER
:SPAN_KIND_PRODUCER rdf:type owl:NamedIndividual ,
                             :SpanKind ;
                    :enumOptionValue "4"^^xsd:int ;
                    rdfs:comment """Indicates that the span describes a producer sending a message to a broker.
Unlike CLIENT and SERVER, there is often no direct critical path latency relationship between producer and consumer spans. A PRODUCER span ends when the message was accepted by the broker while the logical processing of the message might span a much longer time."""@en .


###  https://github.com/andrej-kocijan/opentelemetry-ontology#SPAN_KIND_SERVER
:SPAN_KIND_SERVER rdf:type owl:NamedIndividual ,
                           :SpanKind ;
                  :enumOptionValue "2"^^xsd:int ;
                  rdfs:comment "Indicates that the span covers server-side handling of an RPC or other remote network request."@en .


###  https://github.com/andrej-kocijan/opentelemetry-ontology#SPAN_KIND_UNSPECIFIED
:SPAN_KIND_UNSPECIFIED rdf:type owl:NamedIndividual ,
                                :SpanKind ;
                       :enumOptionValue "0"^^xsd:int ;
                       rdfs:comment """Unspecified. Do NOT use as default.
Implementations MAY assume SpanKind to be INTERNAL when receiving UNSPECIFIED."""@en .


###  https://github.com/andrej-kocijan/opentelemetry-ontology#STATUS_CODE_ERROR
:STATUS_CODE_ERROR rdf:type owl:NamedIndividual ,
                            :StatusCode ;
                   :enumOptionValue "0"^^xsd:int ;
                   rdfs:comment "The Span contains an error."@en .


###  https://github.com/andrej-kocijan/opentelemetry-ontology#STATUS_CODE_OK
:STATUS_CODE_OK rdf:type owl:NamedIndividual ,
                         :StatusCode ;
                :enumOptionValue "1"^^xsd:int ;
                rdfs:comment "The Span has been validated by an Application developer or Operator to have completed successfully."@en .


###  https://github.com/andrej-kocijan/opentelemetry-ontology#STATUS_CODE_UNSET
:STATUS_CODE_UNSET rdf:type owl:NamedIndividual ,
                            :StatusCode ;
                   :enumOptionValue "2"^^xsd:int ;
                   rdfs:comment "The default status."@en .


###  Generated by the OWL API (version 4.5.29.2024-05-13T12:11:03Z) https://github.com/owlcs/owlapi
